vale/code/arch/x64/interop/Vale.AsLowStar.Wrapper.fst
@@ -7,6 +7,7 @@ module UV = LowStar.BufferView.Up
 module DV = LowStar.BufferView.Down
 module HS = FStar.HyperStack
 module ME = X64.Memory
+module SI = X64.Stack_i
 module TS = X64.Taint_Semantics_s
 module MS = X64.Machine_s
 module IA = Interop.Assumptions
@@ -24,17 +25,12 @@ open FStar.Mul
 let lemma_create_initial_vale_state_core
     (#max_arity:nat)
     (#reg_arg:IX64.arg_reg_relation max_arity)
-    (#n:IX64.max_slots)
     (args:IX64.arg_list)
-    (h0:HS.mem)
-    (stack:IX64.stack_buffer n{
-      B.length stack >= n/8 + (List.Tot.length args - max_arity) + 5 /\    
-      mem_roots_p h0 (arg_of_sb stack::args)})
+    (h0:HS.mem{mem_roots_p h0 args})
   : Lemma
       (ensures (
-        let s = LSig.create_initial_vale_state #max_arity #reg_arg args h0 stack in
-        let h1 = IX64.stack_of_args max_arity (List.Tot.length args) args stack h0 in
-        hs_of_mem (as_mem s.VS.mem) == h1
+        let s = LSig.create_initial_vale_state #max_arity #reg_arg args h0 in
+        hs_of_mem (as_mem s.VS.mem) == h0
       ))
   = ()
 
@@ -91,16 +87,12 @@ let arg_is_registered_root (s:ME.mem) (a:arg) =
 let core_create_lemma_readable
     (#max_arity:nat)
     (#arg_reg:IX64.arg_reg_relation max_arity)
-    #n
     (args:IX64.arg_list)
-    (h0:HS.mem)
-    (stack:IX64.stack_buffer n{
-      B.length stack >= n/8 + (List.Tot.length args - max_arity) + 5 /\    
-      mem_roots_p h0 (arg_of_sb stack::args)})
+    (h0:HS.mem{mem_roots_p h0 args})
   : Lemma
       (ensures
-        (let va_s = LSig.create_initial_vale_state #max_arity #arg_reg args h0 stack in
-         VSig.readable (arg_of_sb stack::args) VS.(va_s.mem)))
+        (let va_s = LSig.create_initial_vale_state #max_arity #arg_reg args h0 in
+         VSig.readable args VS.(va_s.mem)))
   =
     let readable_registered_one (a:arg) (s:ME.mem)
       : Lemma
@@ -134,9 +126,7 @@ let core_create_lemma_readable
          FStar.Classical.forall_intro (FStar.Classical.move_requires (args_b8_lemma args));
          readable_registered_all args (as_vale_mem mem)
      in
-     let h1 = IX64.stack_of_args max_arity (List.Tot.length args) args stack h0 in
-     IX64.live_arg_modifies h0 h1 args stack;     
-     readable_mk_mem (arg_of_sb stack::args) h1
+     readable_mk_mem args h0
 
 let readable_live_one (m:ME.mem) (a:arg)
   : Lemma (VSig.readable_one m a ==>
@@ -159,67 +149,38 @@ let rec readable_all_live (m:ME.mem) (args:list arg)
       readable_live_one m hd;
       readable_all_live m tl
 
-let core_create_lemma_readable2
-    (#max_arity:nat)
-    (#arg_reg:IX64.arg_reg_relation max_arity)
-    #n
-    (args:IX64.arg_list)
-    (h0:HS.mem)
-    (stack:IX64.stack_buffer n{
-      B.length stack >= n/8 + (List.Tot.length args - max_arity) + 5 /\    
-      mem_roots_p h0 (arg_of_sb stack::args)})
-  : Lemma
-      (ensures
-        (let va_s = LSig.create_initial_vale_state #max_arity #arg_reg args h0 stack in
-         ME.buffer_readable VS.(va_s.mem) (as_vale_buffer stack) /\
-         VSig.readable args VS.(va_s.mem)))
-  = core_create_lemma_readable #max_arity #arg_reg args h0 stack;
-    let va_s = LSig.create_initial_vale_state #max_arity #arg_reg args h0 stack in
-    readable_cons (arg_of_sb stack) args VS.(va_s.mem)
-
 let core_create_lemma_mem_correspondance
     (#max_arity:nat)
     (#arg_reg:IX64.arg_reg_relation max_arity)
-    #n
     (args:IX64.arg_list)
-    (h0:HS.mem)
-    (stack:IX64.stack_buffer n{
-      B.length stack >= n/8 + (List.Tot.length args - max_arity) + 5 /\    
-      mem_roots_p h0 (arg_of_sb stack::args)})
+    (h0:HS.mem{mem_roots_p h0 args})
   : Lemma
       (ensures
-        (let va_s = LSig.create_initial_vale_state #max_arity #arg_reg args h0 stack in
+        (let va_s = LSig.create_initial_vale_state #max_arity #arg_reg args h0 in
          LSig.mem_correspondence args h0 va_s))
   =
-    let va_s = LSig.create_initial_vale_state #max_arity #arg_reg args h0 stack in
-    let h1 = IX64.stack_of_args max_arity (List.Tot.length args) args stack h0 in    
+    let va_s = LSig.create_initial_vale_state #max_arity #arg_reg args h0 in
     let rec aux (accu:list arg) : Lemma 
-      (requires (forall x. List.memP x accu ==> (
-        disjoint_or_eq_1 (arg_of_sb stack) x /\
-        live_arg h0 x)))
+      (requires (forall x. List.memP x accu ==> (live_arg h0 x)))
       (ensures LSig.mem_correspondence accu h0 va_s) =
     match accu with
     | [] -> ()
     | hd::tl -> aux tl;
-        IX64.live_arg_modifies h0 h1 args stack;      
       match hd with
       | (| TD_Buffer src bt _, x |) ->
-        Vale.AsLowStar.MemoryHelpers.buffer_as_seq_reveal src bt x args h1 stack;
-        Vale.AsLowStar.MemoryHelpers.same_buffer_same_upviews #src #bt x h0 h1;
+        Vale.AsLowStar.MemoryHelpers.buffer_as_seq_reveal src bt x args h0;
         let db = get_downview x in
         DV.length_eq db;
         let ub = UV.mk_buffer db (LSig.view_of_base_typ bt) in
-        assert (Seq.equal (UV.as_seq h0 ub) (UV.as_seq h1 ub))
+        assert (Seq.equal (UV.as_seq h0 ub) (UV.as_seq h0 ub))
       | (| TD_ImmBuffer src bt _, x |) ->
-        Vale.AsLowStar.MemoryHelpers.immbuffer_as_seq_reveal src bt x args h1 stack;
-        Vale.AsLowStar.MemoryHelpers.same_immbuffer_same_upviews #src #bt x h0 h1;
+        Vale.AsLowStar.MemoryHelpers.immbuffer_as_seq_reveal src bt x args h0;
         let db = get_downview x in
         DV.length_eq db;
         let ub = UV.mk_buffer db (LSig.view_of_base_typ bt) in
-        assert (Seq.equal (UV.as_seq h0 ub) (UV.as_seq h1 ub))        
+        assert (Seq.equal (UV.as_seq h0 ub) (UV.as_seq h0 ub))        
       | (| TD_Base _, _ |) -> ()
     in
-    BigOps.big_and'_forall (disjoint_or_eq_1 (arg_of_sb stack)) args;
     BigOps.big_and'_forall (live_arg h0) args;
     aux args
 
@@ -278,21 +239,17 @@ let rec lemma_register_args'
 let core_create_lemma_register_args
     (#max_arity:nat)
     (#arg_reg:IX64.arg_reg_relation max_arity)
-    #n
     (args:IX64.arg_list)
-    (h0:HS.mem)
-    (stack:IX64.stack_buffer n{
-      B.length stack >= n/8 + (List.Tot.length args - max_arity) + 5 /\    
-      mem_roots_p h0 (arg_of_sb stack::args)})
+    (h0:HS.mem{mem_roots_p h0 args})
   : Lemma
-      (ensures (let va_s = LSig.create_initial_vale_state #max_arity #arg_reg args h0 stack in
+      (ensures (let va_s = LSig.create_initial_vale_state #max_arity #arg_reg args h0 in
                 LSig.register_args max_arity arg_reg (List.length args) args va_s))
   =
-    let va_s = LSig.create_initial_vale_state #max_arity #arg_reg args h0 stack in
+    let va_s = LSig.create_initial_vale_state #max_arity #arg_reg args h0 in
     let regs' = IX64.register_of_args max_arity arg_reg (List.Tot.length args) args IA.init_regs in
     lemma_register_args' max_arity arg_reg args IA.init_regs;
     let open MS in
-    let regs = FunctionalExtensionality.on reg (IX64.regs_with_stack regs' stack) in
+    let regs = FunctionalExtensionality.on reg regs' in
     lemma_register_args'_aux max_arity arg_reg (List.length args) args regs' regs;
     assert (register_args' max_arity arg_reg (List.length args) args regs);
     let rec aux
@@ -317,30 +274,25 @@ let core_create_lemma_register_args
         | TD_ImmBuffer src bt _ -> Vale.AsLowStar.MemoryHelpers.immbuffer_addr_reveal src bt x args' h0
         | TD_Base _ -> ()
       in
-      let h1 = IX64.stack_of_args max_arity (List.Tot.length args) args stack h0 in  
-      IX64.live_arg_modifies h0 h1 args stack;      
-      aux args va_s (arg_of_sb stack::args) h1
+      aux args va_s args h0
 
 let core_create_lemma_state
     (#max_arity:nat)
     (#arg_reg:IX64.arg_reg_relation max_arity)
-    #n
     (args:IX64.arg_list)
-    (h0:HS.mem)
-    (stack:IX64.stack_buffer n{
-      B.length stack >= n/8 + (List.Tot.length args - max_arity) + 5 /\
-      mem_roots_p h0 (arg_of_sb stack::args)})
+    (h0:HS.mem{mem_roots_p h0 args})
   : Lemma
       (ensures
-        (let va_s = LSig.create_initial_vale_state #max_arity #arg_reg args h0 stack in
-         fst (IX64.create_initial_trusted_state max_arity arg_reg n args I.down_mem h0 stack) == SL.state_to_S va_s))
-  = let va_s = LSig.create_initial_vale_state #max_arity #arg_reg args h0 stack in
-    let tr_s = fst (IX64.create_initial_trusted_state max_arity arg_reg n args I.down_mem h0 stack) in
+        (let va_s = LSig.create_initial_vale_state #max_arity #arg_reg args h0 in
+         fst (IX64.create_initial_trusted_state max_arity arg_reg args I.down_mem h0) == SL.state_to_S va_s))
+  = let va_s = LSig.create_initial_vale_state #max_arity #arg_reg args h0 in
+    let tr_s = fst (IX64.create_initial_trusted_state max_arity arg_reg args I.down_mem h0) in
     let sl_s = SL.state_to_S va_s in
     assert (tr_s.TS.memTaint == va_s.VS.memTaint);
     SL.lemma_to_ok va_s;
     SL.lemma_to_flags va_s;
     SL.lemma_to_mem va_s;
+    SL.lemma_to_stack va_s;
     let aux_reg (r:MS.reg) : Lemma (tr_s.TS.state.BS.regs r == sl_s.TS.state.BS.regs r)
       = SL.lemma_to_reg va_s r
     in
@@ -351,41 +303,37 @@ let core_create_lemma_state
     Classical.forall_intro aux_xmm;
     assert (FunctionalExtensionality.feq tr_s.TS.state.BS.regs sl_s.TS.state.BS.regs);
     assert (FunctionalExtensionality.feq tr_s.TS.state.BS.xmms sl_s.TS.state.BS.xmms);
-    let h1 = IX64.stack_of_args max_arity (List.Tot.length args) args stack h0 in  
-    IX64.live_arg_modifies h0 h1 args stack;       
-    Vale.AsLowStar.MemoryHelpers.get_heap_mk_mem_reveal args h1 stack
+    Vale.AsLowStar.MemoryHelpers.get_heap_mk_mem_reveal args h0;
+    Vale.AsLowStar.MemoryHelpers.mk_stack_reveal tr_s.TS.state.BS.stack
 
-let rec stack_of_args_equal_domains
-    (#num_b8_slots:_)
-    (max_arity:nat)
-    (n:nat)
-    (args:IX64.arg_list{List.Tot.length args = n})
-    (stack_b:IX64.stack_buffer num_b8_slots
-      {B.length stack_b >= num_b8_slots/8 + (List.Tot.length args - max_arity) + 5 })
-    (h:HS.mem{B.live h stack_b}) : Lemma
-    (ST.equal_domains h (IX64.stack_of_args max_arity n args stack_b h))
-    = match args with
-    | [] -> ()
-    | hd::tl ->
-    if n <= max_arity then ()
-    else 
-      let i = (n - max_arity) - 1 // Arguments on the stack are pushed from right to left
-        + (if IA.win then 4 else 0) // The shadow space on Windows comes next
-        + 1 // The return address is then pushed on the stack
-        + num_b8_slots / 8 // And we then have all the extra slots required for the Vale procedure
-      in
-      let h1 = IX64.stack_of_args max_arity (n-1) tl stack_b h in      
-      let v = UInt64.uint_to_t (IX64.arg_as_nat64 hd) in // We will store the arg hd
-      B.g_upd_seq_as_seq stack_b (Seq.upd (B.as_seq h1 stack_b) i v) h1;
-      stack_of_args_equal_domains max_arity (n-1) tl stack_b h
+// let rec stack_of_args_equal_domains
+//     (#num_b8_slots:_)
+//     (max_arity:nat)
+//     (n:nat)
+//     (args:IX64.arg_list{List.Tot.length args = n})
+//     (h:HS.mem) : Lemma
+//     (ST.equal_domains h (IX64.stack_of_args max_arity n args stack_b h))
+//     = match args with
+//     | [] -> ()
+//     | hd::tl ->
+//     if n <= max_arity then ()
+//     else 
+//       let i = (n - max_arity) - 1 // Arguments on the stack are pushed from right to left
+//         + (if IA.win then 4 else 0) // The shadow space on Windows comes next
+//         + 1 // The return address is then pushed on the stack
+//         + num_b8_slots / 8 // And we then have all the extra slots required for the Vale procedure
+//       in
+//       let h1 = IX64.stack_of_args max_arity (n-1) tl stack_b h in      
+//       let v = UInt64.uint_to_t (IX64.arg_as_nat64 hd) in // We will store the arg hd
+//       B.g_upd_seq_as_seq stack_b (Seq.upd (B.as_seq h1 stack_b) i v) h1;
+//       stack_of_args_equal_domains max_arity (n-1) tl stack_b h
 
+(*
 let rec stack_args' (max_arity:nat)
                    (num_b8_slots:IX64.max_slots)
                    (n:nat)
                    (args:list arg{List.Tot.length args = n})
                    (h0:HS.mem)
-                   (stack_b:IX64.stack_buffer num_b8_slots
-                      {B.length stack_b >= num_b8_slots/8 + (List.Tot.length args - max_arity) + 5 })
                    : prop =
     match args with
     | [] -> True
@@ -405,8 +353,6 @@ let rec stack_of_args_stack_args'
     (max_arity:nat)
     (n:nat)
     (args:IX64.arg_list{List.Tot.length args = n})
-    (stack_b:IX64.stack_buffer num_b8_slots
-      {B.length stack_b >= num_b8_slots/8 + (List.Tot.length args - max_arity) + 5 })
     (h0:HS.mem{B.live h0 stack_b}) : Lemma
     (stack_args' max_arity num_b8_slots n args (IX64.stack_of_args max_arity n args stack_b h0) stack_b)
     = match args with
@@ -433,160 +379,137 @@ let rec stack_of_args_stack_args'
       | [] -> ()
       | hd::tl -> aux tl
       in aux tl
+*)
 
 let core_create_lemma_stack_args
     (#max_arity:nat)
     (#arg_reg:IX64.arg_reg_relation max_arity)
-    #n
     (args:IX64.arg_list)
-    (h0:HS.mem)
-    (stack:IX64.stack_buffer n{
-      B.length stack >= n/8 + (List.Tot.length args - max_arity) + 5 /\    
-      mem_roots_p h0 (arg_of_sb stack::args)})
+    (h0:HS.mem{mem_roots_p h0 args})
   : Lemma
-      (ensures (let va_s = LSig.create_initial_vale_state #max_arity #arg_reg args h0 stack in
-                LSig.stack_args max_arity n (List.length args) args stack va_s))
-  =
-    let va_s = LSig.create_initial_vale_state #max_arity #arg_reg args h0 stack in
-    let h1 = IX64.stack_of_args max_arity (List.Tot.length args) args stack h0 in
-    IX64.live_arg_modifies h0 h1 args stack;
-    assert (mem_roots_p h1 (arg_of_sb stack::args));   
-    let rec aux (accu:IX64.arg_list{List.length accu <= List.length args}) : Lemma
-      (requires 
-        mem_roots_p h1 (arg_of_sb stack::args) /\
-        stack_args' max_arity n (List.length accu) accu h1 stack)
-      (ensures LSig.stack_args max_arity n (List.length accu) accu stack va_s)
-    = match accu with
-      | [] -> ()
-      | hd::tl -> aux tl;
-        let i = List.length accu in
-        if i <= max_arity then ()
-        else (
-          let j = (i - max_arity) - 1 + (if IA.win then 4 else 0) + 1 + n/8 in
-          assert (UInt64.v (B.get h1 stack j) == IX64.arg_as_nat64 hd);
-          DV.length_eq (get_downview stack);
-          let aux2 () : Lemma (IX64.arg_as_nat64 hd == LSig.arg_as_nat64 hd va_s) =
-            match hd with
-            | (| TD_Buffer src bt _, x |) ->
-              Vale.AsLowStar.MemoryHelpers.buffer_addr_reveal src bt x (arg_of_sb stack::args) h1
-            | (| TD_ImmBuffer src bt _, x |) ->              
-              Vale.AsLowStar.MemoryHelpers.immbuffer_addr_reveal src bt x (arg_of_sb stack::args) h1
-            | _ -> ()
-          in aux2();
-          Vale.AsLowStar.MemoryHelpers.buffer_as_seq_reveal2 TUInt64 TUInt64 stack va_s;
-          Vale.AsLowStar.MemoryHelpers.down_up_buffer_read_reveal TUInt64 h1 va_s.VS.mem stack j
-        )
-    in
-    stack_of_args_stack_args' max_arity (List.length args) args stack h0;
-    aux args
+      (ensures (let va_s = LSig.create_initial_vale_state #max_arity #arg_reg args h0 in
+                LSig.stack_args max_arity (List.length args) args va_s))
+  = admit()
+    // let va_s = LSig.create_initial_vale_state #max_arity #arg_reg args h0 in
+    // // let h1 = IX64.stack_of_args max_arity (List.Tot.length args) args h0 in
+    // // IX64.live_arg_modifies h0 h1 args stack;
+    // // assert (mem_roots_p h1 (arg_of_sb stack::args));   
+    // let rec aux (accu:IX64.arg_list{List.length accu <= List.length args}) : Lemma
+    //   (requires 
+    //     mem_roots_p h1 (arg_of_sb stack::args) /\
+    //     stack_args' max_arity n (List.length accu) accu h1 stack)
+    //   (ensures LSig.stack_args max_arity n (List.length accu) accu stack va_s)
+    // = match accu with
+    //   | [] -> ()
+    //   | hd::tl -> aux tl;
+    //     let i = List.length accu in
+    //     if i <= max_arity then ()
+    //     else (
+    //       let j = (i - max_arity) - 1 + (if IA.win then 4 else 0) + 1 + n/8 in
+    //       assert (UInt64.v (B.get h1 stack j) == IX64.arg_as_nat64 hd);
+    //       DV.length_eq (get_downview stack);
+    //       let aux2 () : Lemma (IX64.arg_as_nat64 hd == LSig.arg_as_nat64 hd va_s) =
+    //         match hd with
+    //         | (| TD_Buffer src bt _, x |) ->
+    //           Vale.AsLowStar.MemoryHelpers.buffer_addr_reveal src bt x (arg_of_sb stack::args) h1
+    //         | (| TD_ImmBuffer src bt _, x |) ->              
+    //           Vale.AsLowStar.MemoryHelpers.immbuffer_addr_reveal src bt x (arg_of_sb stack::args) h1
+    //         | _ -> ()
+    //       in aux2();
+    //       Vale.AsLowStar.MemoryHelpers.buffer_as_seq_reveal2 TUInt64 TUInt64 stack va_s;
+    //       Vale.AsLowStar.MemoryHelpers.down_up_buffer_read_reveal TUInt64 h1 va_s.VS.mem stack j
+    //     )
+    // in
+    // stack_of_args_stack_args' max_arity (List.length args) args stack h0;
+    // aux args
 
 
 let core_create_lemma
     (#max_arity:nat)
     (#arg_reg:IX64.arg_reg_relation max_arity)
-    #n
     (args:IX64.arg_list)
-    (h0:HS.mem)
-    (stack:IX64.stack_buffer n{
-      B.length stack >= n/8 + (List.Tot.length args - max_arity) + 5 /\
-      mem_roots_p h0 (arg_of_sb stack::args)})
+    (h0:HS.mem{mem_roots_p h0 args})
   : Lemma
       (ensures
-        (let va_s = LSig.create_initial_vale_state #max_arity #arg_reg args h0 stack in
-         fst (IX64.create_initial_trusted_state max_arity arg_reg n args I.down_mem h0 stack) == SL.state_to_S va_s /\
+        (let va_s = LSig.create_initial_vale_state #max_arity #arg_reg args h0 in
+         fst (IX64.create_initial_trusted_state max_arity arg_reg args I.down_mem h0) == SL.state_to_S va_s /\
          LSig.mem_correspondence args h0 va_s /\
-         VSig.disjoint_or_eq (arg_of_sb stack :: args) /\
+         VSig.disjoint_or_eq args /\
          VSig.readable args VS.(va_s.mem) /\
-         LSig.vale_pre_hyp #max_arity #arg_reg args stack va_s /\
-         ST.equal_domains h0 (hs_of_mem (as_mem va_s.VS.mem)) /\
-         V.valid_stack_slots
-                va_s.VS.mem
-                (VS.eval_reg MS.Rsp va_s)
-                (as_vale_buffer stack)
-                (n / 8)
-                va_s.VS.memTaint
+         LSig.vale_pre_hyp #max_arity #arg_reg args va_s /\
+         ST.equal_domains h0 (hs_of_mem (as_mem va_s.VS.mem))
   ))
   =  
-  let va_s = LSig.create_initial_vale_state #max_arity #arg_reg args h0 stack in
-    core_create_lemma_mem_correspondance #max_arity #arg_reg args h0 stack;
-    core_create_lemma_disjointness (arg_of_sb stack :: args);
-    core_create_lemma_readable #max_arity #arg_reg args h0 stack;
-    core_create_lemma_readable2 #max_arity #arg_reg args h0 stack;
-    core_create_lemma_register_args #max_arity #arg_reg args h0 stack;
-    core_create_lemma_stack_args #max_arity #arg_reg args h0 stack;
-    Vale.AsLowStar.MemoryHelpers.core_create_lemma_taint_hyp #max_arity #arg_reg args h0 stack;
-    core_create_lemma_state #max_arity #arg_reg args h0 stack;
-    Vale.AsLowStar.MemoryHelpers.buffer_writeable_reveal ME.TUInt64 ME.TUInt64 stack;
-    let s_args = arg_of_sb stack :: args in
-    let h1 = IX64.stack_of_args max_arity (List.Tot.length args) args stack h0 in  
-    stack_of_args_equal_domains max_arity (List.Tot.length args) args stack h0;
-    IX64.live_arg_modifies h0 h1 args stack;           
-    Vale.AsLowStar.MemoryHelpers.buffer_addr_reveal _ _ stack (arg_of_sb stack :: args) h1;
-    DV.length_eq (get_downview stack);
-    Vale.AsLowStar.MemoryHelpers.as_vale_buffer_len stack;
-    FStar.Math.Lemmas.lemma_div_le n (B.length stack * 8) 8
+  let va_s = LSig.create_initial_vale_state #max_arity #arg_reg args h0 in
+    core_create_lemma_mem_correspondance #max_arity #arg_reg args h0;
+    core_create_lemma_disjointness args;
+    core_create_lemma_readable #max_arity #arg_reg args h0;
+    core_create_lemma_register_args #max_arity #arg_reg args h0;
+    core_create_lemma_stack_args #max_arity #arg_reg args h0;
+    Vale.AsLowStar.MemoryHelpers.core_create_lemma_taint_hyp #max_arity #arg_reg args h0;
+    core_create_lemma_state #max_arity #arg_reg args h0
 
-let rec frame_mem_correspondence_back
-       (args:list arg)
-       (h0:mem_roots args)
-       (h1:mem_roots args)
-       (va_s:V.va_state)
-       (l:B.loc)
- : Lemma
-     (requires
-       LSig.mem_correspondence args h1 va_s /\
-       B.modifies l h0 h1 /\
-       B.loc_disjoint (loc_all_args args) l)
-     (ensures
-       LSig.mem_correspondence args h0 va_s)
- = match args with
-   | [] -> ()
-   | hd::tl ->
-     frame_mem_correspondence_back tl h0 h1 va_s l;
-     match hd with
-     | (| TD_Buffer src bt _, x |) | (| TD_ImmBuffer src bt _, x |) ->
-       BufferViewHelpers.lemma_dv_equal (down_view src) x h0 h1;
-       DV.length_eq (get_downview x);
-       BufferViewHelpers.lemma_uv_equal (LSig.view_of_base_typ bt) (get_downview x) h0 h1
-     | (| TD_Base _, _ |) -> ()
+// let rec frame_mem_correspondence_back
+//        (args:list arg)
+//        (h0:mem_roots args)
+//        (h1:mem_roots args)
+//        (va_s:V.va_state)
+//        (l:B.loc)
+//  : Lemma
+//      (requires
+//        LSig.mem_correspondence args h1 va_s /\
+//        B.modifies l h0 h1 /\
+//        B.loc_disjoint (loc_all_args args) l)
+//      (ensures
+//        LSig.mem_correspondence args h0 va_s)
+//  = match args with
+//    | [] -> ()
+//    | hd::tl ->
+//      frame_mem_correspondence_back tl h0 h1 va_s l;
+//      match hd with
+//      | (| TD_Buffer src bt _, x |) | (| TD_ImmBuffer src bt _, x |) ->
+//        BufferViewHelpers.lemma_dv_equal (down_view src) x h0 h1;
+//        DV.length_eq (get_downview x);
+//        BufferViewHelpers.lemma_uv_equal (LSig.view_of_base_typ bt) (get_downview x) h0 h1
+//      | (| TD_Base _, _ |) -> ()
 
-let rec frame_mem_correspondence
-       (args:list arg)
-       (h0:mem_roots args)
-       (h1:HS.mem)
-       (va_s:V.va_state)
-       (l:B.loc)
- : Lemma
-     (requires
-       LSig.mem_correspondence args h0 va_s /\
-       B.modifies l h0 h1 /\
-       B.loc_disjoint (loc_all_args args) l)
-     (ensures
-       LSig.mem_correspondence args h1 va_s /\
-       mem_roots_p h1 args)
- = match args with
-   | [] -> ()
-   | hd::tl ->
-     frame_mem_correspondence tl h0 h1 va_s l;
-     match hd with
-     | (| TD_Buffer src bt _, x |) | (| TD_ImmBuffer src bt _, x |) ->
-       BufferViewHelpers.lemma_dv_equal (down_view src) x h0 h1;
-       DV.length_eq (get_downview x);
-       BufferViewHelpers.lemma_uv_equal (LSig.view_of_base_typ bt) (get_downview x) h0 h1     
-     | (| TD_Base _, _ |) -> ()
+// let rec frame_mem_correspondence
+//        (args:list arg)
+//        (h0:mem_roots args)
+//        (h1:HS.mem)
+//        (va_s:V.va_state)
+//        (l:B.loc)
+//  : Lemma
+//      (requires
+//        LSig.mem_correspondence args h0 va_s /\
+//        B.modifies l h0 h1 /\
+//        B.loc_disjoint (loc_all_args args) l)
+//      (ensures
+//        LSig.mem_correspondence args h1 va_s /\
+//        mem_roots_p h1 args)
+//  = match args with
+//    | [] -> ()
+//    | hd::tl ->
+//      frame_mem_correspondence tl h0 h1 va_s l;
+//      match hd with
+//      | (| TD_Buffer src bt _, x |) | (| TD_ImmBuffer src bt _, x |) ->
+//        BufferViewHelpers.lemma_dv_equal (down_view src) x h0 h1;
+//        DV.length_eq (get_downview x);
+//        BufferViewHelpers.lemma_uv_equal (LSig.view_of_base_typ bt) (get_downview x) h0 h1     
+//      | (| TD_Base _, _ |) -> ()
 
-let rec args_fp (args:list arg)
-                (h0:mem_roots args)
-                (h1:HS.mem{HS.fresh_frame h0 h1})
-  : Lemma
-      (B.loc_disjoint (loc_all_args args) (B.loc_regions false (Set.singleton (HS.get_tip h1))))
-  = match args with
-    | [] -> ()
-    | hd::tl -> args_fp tl h0 h1; 
-      match hd with
-      | (| TD_Buffer _ _ _, _ |) | (| TD_Base _, _ |) -> ()
-      | (| TD_ImmBuffer _ _ _, x |) -> 
-        assert (B.loc_includes (B.loc_not_unused_in h0) (B.loc_buffer x))
+// let rec args_fp (args:list arg)
+//                 (h0:mem_roots args)
+//                 (h1:HS.mem{HS.fresh_frame h0 h1})
+//   : Lemma
+//       (B.loc_disjoint (loc_all_args args) (B.loc_regions false (Set.singleton (HS.get_tip h1))))
+//   = match args with
+//     | [] -> ()
+//     | hd::tl -> args_fp tl h0 h1; 
+//       match hd with
+//       | (| TD_Buffer _ _ _, _ |) | (| TD_Base _, _ |) -> ()
+//       | (| TD_ImmBuffer _ _ _, x |) -> 
+//         assert (B.loc_includes (B.loc_not_unused_in h0) (B.loc_buffer x))
 
 let eval_code_ts (c:TS.tainted_code)
                  (s0:TS.traceState)
@@ -624,8 +547,7 @@ let rec mem_correspondence_refl (args:list arg)
 let prediction_pre_rel
           (#max_arity:nat)
           (#arg_reg:IX64.arg_reg_relation max_arity)
-          (#n:IX64.max_slots)
-          (pre:VSig.vale_pre_tl n [])
+          (pre:VSig.vale_pre_tl [])
           (code:V.va_code)
           (args:IX64.arg_list)
    : IX64.prediction_pre_rel_t code args
@@ -635,29 +557,19 @@ let prediction_pre_rel
 [@__reduce__]
 let prediction_post_rel
           (#max_arity:nat)
-          #n
-          (post:VSig.vale_post_tl n [])
+          (post:VSig.vale_post_tl [])
           (code:V.va_code)
           (args:IX64.arg_list)
-   : IX64.prediction_post_rel_t code n args
+   : IX64.prediction_post_rel_t code args
    = fun (h0:mem_roots args)
        (_s0:TS.traceState)
-       (_push_h0:mem_roots args)
-       (_alloc_push_h0:mem_roots args)
-       (_sb:IX64.stack_buffer n)
        (rax_fuel_mem:(UInt64.t & nat & ME.mem))
        (s1:TS.traceState) ->
     let rax, fuel, mem = rax_fuel_mem in
-    exists h1_pre_pop.
-      h1_pre_pop == hs_of_mem (as_mem mem) /\
-      HS.poppable h1_pre_pop /\ (
-      exists h1. h1 == HS.pop h1_pre_pop /\
-        mem_roots_p h1 args /\
-        LSig.(to_low_post post args h0 rax h1))
-
-let pop_is_popped (m:HS.mem{HS.poppable m})
-  : Lemma (HS.popped m (HS.pop m))
-  = ()
+    exists h1.
+      h1 == hs_of_mem (as_mem mem) /\
+      mem_roots_p h1 args /\
+      LSig.(to_low_post post args h0 rax h1)
 
 let loc_includes_union (l1 l1' l:B.loc)
   : Lemma (requires B.(loc_includes l1 l1'))
@@ -673,11 +585,10 @@ val vale_lemma_as_prediction
           (#arg_reg:IX64.arg_reg_relation max_arity)
           (#regs_modified:MS.reg -> bool)
           (#xmms_modified:MS.xmm -> bool)          
-          (#n:IX64.max_slots)
           (code:V.va_code)
           (args:IX64.arg_list)
-          (pre:VSig.vale_pre_tl n [])
-          (post:VSig.vale_post_tl n [])
+          (pre:VSig.vale_pre_tl [])
+          (post:VSig.vale_post_tl [])
           (v:VSig.vale_sig_tl regs_modified xmms_modified args (coerce code) pre post)
    : IX64.prediction
              max_arity
@@ -686,7 +597,6 @@ val vale_lemma_as_prediction
              xmms_modified
              I.down_mem
              (coerce code)
-             n
              args
              (prediction_pre_rel #max_arity #arg_reg pre (coerce code) args)
              (prediction_post_rel #max_arity post (coerce code) args)
@@ -696,78 +606,57 @@ let vale_lemma_as_prediction
           (#arg_reg:IX64.arg_reg_relation max_arity)
           (#regs_modified:MS.reg -> bool)
           (#xmms_modified:MS.xmm -> bool)
-          (#n:IX64.max_slots)
           (code:V.va_code)
           (args:IX64.arg_list)
-          (pre:VSig.vale_pre_tl n [])
-          (post:VSig.vale_post_tl n [])
+          (pre:VSig.vale_pre_tl [])
+          (post:VSig.vale_post_tl [])
           (v:VSig.vale_sig_tl regs_modified xmms_modified args (coerce code) pre post)
-   = fun h0 s0 push_h0 alloc_push_h0 sb ->
+   = fun h0 s0 ->
        let c_code : TS.tainted_code = coerce code in
-       let s_args = arg_of_sb sb :: args in
-       let va_s0 = LSig.create_initial_vale_state #max_arity #arg_reg args alloc_push_h0 sb in
-       core_create_lemma #max_arity #arg_reg args alloc_push_h0 sb;
+       let va_s0 = LSig.create_initial_vale_state #max_arity #arg_reg args h0 in
+       core_create_lemma #max_arity #arg_reg args h0;
        assert (SL.state_to_S va_s0 == s0);
-       B.fresh_frame_modifies h0 push_h0;
-       assert (B.modifies B.loc_none h0 alloc_push_h0);
-       assert (LSig.mem_correspondence args alloc_push_h0 va_s0);
-       frame_mem_correspondence_back args h0 alloc_push_h0 va_s0 B.loc_none;
        assert (LSig.mem_correspondence args h0 va_s0);
        assert (va_s0.VS.ok);
-       assert (LSig.vale_pre_hyp #max_arity #arg_reg args sb va_s0);
-       assert (elim_nil pre va_s0 sb);
-       let va_s1, f = VSig.elim_vale_sig_nil v va_s0 sb in
+       assert (LSig.vale_pre_hyp #max_arity #arg_reg args va_s0);
+       assert (elim_nil pre va_s0);
+       let va_s1, f = VSig.elim_vale_sig_nil v va_s0 in
        assert (V.eval_code code va_s0 f va_s1);
        eval_code_rel (c_code) va_s0 va_s1 f;
        let Some s1 = TS.taint_eval_code (c_code) (coerce f) s0 in
        assert (VL.state_eq_opt (Some (SL.state_to_S va_s1)) (Some s1));
        assert (VSig.vale_calling_conventions va_s0 va_s1 regs_modified xmms_modified);
        assert (IX64.calling_conventions s0 s1 regs_modified xmms_modified);
-       assert (ME.modifies (VSig.mloc_modified_args s_args) va_s0.VS.mem va_s1.VS.mem);
+       assert (ME.modifies (VSig.mloc_modified_args args) va_s0.VS.mem va_s1.VS.mem);
        let final_mem = va_s1.VS.mem in
-       let h1_pre_pop = hs_of_mem (as_mem final_mem) in
-       Vale.AsLowStar.MemoryHelpers.relate_modifies s_args va_s0.VS.mem va_s1.VS.mem;
-       assert (B.modifies (loc_modified_args s_args) alloc_push_h0 h1_pre_pop);
+       let h1= hs_of_mem (as_mem final_mem) in
+       Vale.AsLowStar.MemoryHelpers.relate_modifies args va_s0.VS.mem va_s1.VS.mem;
+       assert (B.modifies (loc_modified_args args) h0 h1);
        Vale.AsLowStar.MemoryHelpers.modifies_equal_domains
-         (VSig.mloc_modified_args s_args) va_s0.VS.mem final_mem;       
+         (VSig.mloc_modified_args args) va_s0.VS.mem final_mem;       
        Vale.AsLowStar.MemoryHelpers.modifies_same_roots 
-         (VSig.mloc_modified_args s_args) va_s0.VS.mem final_mem;
+         (VSig.mloc_modified_args args) va_s0.VS.mem final_mem;
        Vale.AsLowStar.MemoryHelpers.state_eq_down_mem va_s1 s1;
        assert (I.down_mem (as_mem final_mem) == s1.TS.state.BS.mem);
        mem_correspondence_refl args va_s1;
-       assert (HS.poppable h1_pre_pop);
-       let h2 = HS.pop h1_pre_pop in
-       args_fp args h0 push_h0;
-       assert (HS.get_tip push_h0 == HS.get_tip h1_pre_pop);
-       pop_is_popped h1_pre_pop;
-       assert (HS.popped h1_pre_pop h2);
-       B.popped_modifies h1_pre_pop h2;
        assert (VSig.readable args VS.(va_s1.mem));
        assert (disjoint_or_eq args);
        readable_all_live VS.(va_s1.mem) args;
-       assert (all_live h1_pre_pop args);
-       assert (mem_roots_p h1_pre_pop args);
-       frame_mem_correspondence args h1_pre_pop h2 va_s1 (B.loc_regions false (Set.singleton (HS.get_tip h1_pre_pop)));
-       assert (B.modifies (loc_modified_args s_args) alloc_push_h0 h1_pre_pop);
-       assert (B.modifies (loc_modified_args s_args) push_h0 h1_pre_pop);
-       let l = (B.loc_all_regions_from false (HS.get_tip push_h0)) in
-       assert (B.loc_includes l (B.loc_buffer sb));
-       loc_includes_union l (B.loc_buffer sb) (loc_modified_args args);
-       B.modifies_fresh_frame_popped h0 push_h0 (loc_modified_args args) h1_pre_pop h2;
-       assert (B.modifies (loc_modified_args args) h0 h2);
-       assert (LSig.(to_low_post post args h0 (IX64.return_val s1) h2));
+       assert (all_live h1 args);
+       assert (mem_roots_p h1 args);
+       assert (B.modifies (loc_modified_args args) h0 h1);
+       assert (LSig.(to_low_post post args h0 (IX64.return_val s1) h1));
        IX64.return_val s1, coerce f, as_mem va_s1.VS.mem
 
 [@__reduce__]
 let rec lowstar_typ
           (#max_arity:nat)
           (#arg_reg:IX64.arg_reg_relation max_arity)
-          #n
           (#dom:list td)
           (code:V.va_code)
           (args:IX64.arg_list{List.length args + List.length dom <= 20})
-          (pre:VSig.vale_pre_tl n dom)
-          (post:VSig.vale_post_tl n dom)
+          (pre:VSig.vale_pre_tl dom)
+          (post:VSig.vale_post_tl dom)
     : Type =
     let open FStar.HyperStack.ST in
     match dom with
@@ -786,7 +675,6 @@ let rec lowstar_typ
       lowstar_typ
         #max_arity
         #arg_reg
-        #n
         #tl
         code
         ((| hd, x |)::args)
@@ -800,12 +688,11 @@ let rec __test__wrap
              (#arg_reg:IX64.arg_reg_relation max_arity)
              (#regs_modified:MS.reg -> bool)
              (#xmms_modified:MS.xmm -> bool)
-             #n (#dom:list td)
+             (#dom:list td)
              (code:V.va_code)
              (args:list arg{List.length dom + List.length args <= 20})
-             (num_stack_slots:nat)
-             (pre:VSig.vale_pre_tl n dom)
-             (post:VSig.vale_post_tl n dom)
+             (pre:VSig.vale_pre_tl dom)
+             (post:VSig.vale_post_tl dom)
              (v:VSig.vale_sig_tl regs_modified xmms_modified args (coerce code) pre post)
     : lowstar_typ code args pre post =
     match dom with
@@ -822,11 +709,11 @@ let rec __test__wrap
          fun () ->
            let h0 = ST.get () in
            let prediction =
-             vale_lemma_as_prediction _ _ _ _ v in
-           let rax, _ = IX64.wrap_variadic (coerce code) max_arity arg_reg regs_modified xmms_modified I.down_mem n args prediction in
+             vale_lemma_as_prediction code args pre post v in
+           let rax, ret = IX64.wrap_variadic (coerce code) max_arity arg_reg regs_modified xmms_modified I.down_mem args prediction in
            rax
       in
-      f <: lowstar_typ #max_arity #arg_reg #n #[] code args pre post
+      f <: lowstar_typ #max_arity #arg_reg #[] code args pre post
     | hd::tl ->
       fun (x:td_as_type hd) ->
         __test__wrap
@@ -834,7 +721,6 @@ let rec __test__wrap
           #arg_reg
           code
           IX64.(x ++ args)
-          num_stack_slots
           (elim_1 pre x)
           (elim_1 post x)
           (VSig.elim_vale_sig_cons hd tl args pre post v x)
@@ -846,11 +732,10 @@ let rec __test__wrap
 let rec pre_rel_generic
       (#max_arity:nat)
       (#arg_reg:IX64.arg_reg_relation max_arity)
-      (#n:_)
       (code:V.va_code)
       (dom:list td)
       (args:list arg{List.length dom + List.length args <= 20})
-      (pre:VSig.vale_pre_tl n dom)
+      (pre:VSig.vale_pre_tl dom)
    : IX64.rel_gen_t code dom args (IX64.prediction_pre_rel_t (coerce code))
    = match dom with
      | [] ->
@@ -862,12 +747,11 @@ let rec pre_rel_generic
 [@__reduce__]
 let rec post_rel_generic
       (#max_arity:nat)
-      (#n:_)
       (code:V.va_code)
       (dom:list td)
       (args:list arg{List.length dom + List.length args <= 20})
-      (post:VSig.vale_post_tl n dom)
-   : IX64.rel_gen_t code dom args (IX64.prediction_post_rel_t (coerce code) n)
+      (post:VSig.vale_post_tl dom)
+   : IX64.rel_gen_t code dom args (IX64.prediction_post_rel_t (coerce code))
    = match dom with
      | [] ->
        prediction_post_rel #max_arity post (coerce code) args
@@ -880,12 +764,11 @@ let rec mk_prediction
        (#arg_reg:IX64.arg_reg_relation max_arity)
        (#regs_modified:MS.reg -> bool)
        (#xmms_modified:MS.xmm -> bool)
-       #n
        (code:V.va_code)
        (dom:list td)
        (args:list arg{List.length dom + List.length args <= 20})
-       (#pre:VSig.vale_pre_tl n dom)
-       (#post:VSig.vale_post_tl n dom)
+       (#pre:VSig.vale_pre_tl dom)
+       (#post:VSig.vale_post_tl dom)
        (v:VSig.vale_sig_tl regs_modified xmms_modified args (coerce code) pre post)
    :  IX64.prediction_t
           max_arity
@@ -894,7 +777,6 @@ let rec mk_prediction
           xmms_modified
           I.down_mem
           (coerce code)
-          n
           dom
           args
           (pre_rel_generic #max_arity #arg_reg code dom args pre)
